TransVal/Terminates.v
@@ -1,0 +1,19 @@
+Require Import IL smt.
+
+Set Implicit Arguments.
+
+Inductive Terminates :F.state -> F.state -> Prop :=
+|TerminatesReturn L E e v:
+(*   translateExp e = ⎣b⎦  *)
+   exp_eval E e = ⎣v⎦
+   -> Terminates (L, E, stmtReturn e)   (L  , E , stmtReturn e)
+|TerminatesStep sigma sigma' sigma'' a:
+   F.step sigma a sigma'
+   -> Terminates sigma' sigma''
+   -> Terminates sigma sigma''.
+
+(*
+*** Local Variables: ***
+*** coq-load-path: (("../" "Lvc")) ***
+*** End: ***
+*)
