TransVal/transval.v
@@ -1,21 +1,5 @@
 Require Import List.
-Require Import IL Annotation AutoIndTac Bisim Exp MoreExp Coherence Fresh sexp smt nofun terminates bitvec OutVars.
-
-Lemma ssa_impl_eq_val:
-forall x (e:exp) s E E' s' D v,
-terminates (nil, E, stmtExp x e s) (nil, E', s')
-->ssa (stmtExp x e s) D
--> exp_eval E e = Some v
--> E' x = Some v.
-
-Proof.
-admit.
-(*intros. general induction s. 
-inversion H. inversion H2. rewrite <-  H12 in *. clear H12.
-- unfold update. rewrite H1 in def. rewrite def. decide (x===x).
-  + reflexivity.
-  + exfalso; eapply n; reflexivity.
-- *)
+Require Import IL Annotation AutoIndTac Bisim Exp MoreExp Coherence Fresh sexp smt nofun Terminates bitvec OutVars SetOperations Sim.
 
 Lemma zext_nil_eq_O:
 forall k, zext k nil = zext k (O::nil).
@@ -35,20 +19,20 @@ Qed.
 Lemma not_zero_implies_uneq:
 forall a b k, bvZero a = false ->b = zext k (O::nil) ->  val2bool(bvEq a b) -> False.
 
-Proof. 
+Proof.
 intros. general induction a.
 -  destruct a.
    + specialize (IHa (tl (zext k (O::nil))) (k-1)).   simpl in H. specialize (IHa H).  eapply IHa.
      * destruct k; eauto.
        simpl. rewrite zext_nil_eq_O.   erewrite minus_n_0. reflexivity. 
      * destruct k; eauto. simpl in H1.  exfalso. assumption. 
-   +  simpl in H1.destruct k;  assumption. 
+   +  simpl in H1. destruct k;  assumption. 
 Qed.
 
  Lemma guard_true_if_eval:
-forall F E e s v,  
- exp_eval E e = Some v 
-->  undef e = Some s 
+forall F E e s v,
+ exp_eval E e = Some v
+->  undef e = Some s
 ->  models F E s.
 
 Proof.
@@ -56,7 +40,7 @@ intros. general induction e; simpl.
 - simpl in *. monad_inv H. destruct u.
   + apply (IHe F E s x); eauto.
   + destruct u.
-    *  apply (IHe F E s x); eauto. 
+    *  apply (IHe F E s x); eauto.
     * exfalso; discriminate H0.
 - simpl in H.  monad_inv H.  simpl in H0. destruct b.
   +  case_eq (undef e1); case_eq (undef e2); intros.
@@ -69,24 +53,24 @@ intros. general induction e; simpl.
   + destruct b.
     *  case_eq (undef e1); case_eq (undef e2); intros.
      {  rewrite H in H0; rewrite H1 in H0. simpl in H0. inversion H0. simpl; split.
-        - eapply IHe1; eauto. 
+        - eapply IHe1; eauto.
         - eapply IHe2; eauto. }
      { rewrite H in H0; rewrite H1 in H0; simpl in H0; inversion H0; simpl. eapply IHe1; eauto. rewrite <- H0; eauto. }
      { rewrite H in H0; rewrite H1 in H0; simpl in H0; inversion H0; simpl. eapply IHe2; eauto. rewrite <- H0; eauto. }
      { rewrite H in H0; rewrite H1 in H0; simpl in H0;  simpl. exfalso; discriminate H0. }
-    * destruct b. 
+    * destruct b.
       { case_eq (undef e1); case_eq (undef e2); intros.
         -  rewrite H in H0; rewrite H1 in H0. simpl in H0. inversion H0. simpl; split.
-           + eapply IHe1; eauto. 
-           + eapply IHe2; eauto. 
+           + eapply IHe1; eauto.
+           + eapply IHe2; eauto.
         - rewrite H in H0; rewrite H1 in H0; simpl in H0; inversion H0; simpl. eapply IHe1; eauto. rewrite <- H0; eauto.
         - rewrite H in H0; rewrite H1 in H0; simpl in H0; inversion H0; simpl. eapply IHe2; eauto. rewrite <- H0; eauto.
         - rewrite H in H0; rewrite H1 in H0; simpl in H0;  simpl. exfalso; discriminate H0. }
-      { destruct b. 
+      { destruct b.
         -  case_eq (undef e1); case_eq (undef e2); intros.
            +  rewrite H in H0; rewrite H1 in H0. simpl in H0. inversion H0. simpl; split.
-              * eapply IHe1; eauto. 
-              * eapply IHe2; eauto. 
+              * eapply IHe1; eauto.
+              * eapply IHe2; eauto.
            + rewrite H in H0; rewrite H1 in H0; simpl in H0; inversion H0; simpl. eapply IHe1; eauto. rewrite <- H0; eauto.
            + rewrite H in H0; rewrite H1 in H0; simpl in H0; inversion H0; simpl. eapply IHe2; eauto. rewrite <- H0; eauto.
             +rewrite H in H0; rewrite H1 in H0; simpl in H0;  simpl. exfalso; discriminate H0.
@@ -102,28 +86,28 @@ intros. general induction e; simpl.
             * case_eq (undef e1); case_eq (undef e2); intros.
               {  rewrite H in H0; rewrite H1 in H0. simpl in H0. inversion H0.  unfold binop_eval in EQ2.  clear H0. unfold bvDiv in EQ2. simpl. split.
                  - case_eq(bvZero x0).
-                   + intros.  rewrite H0 in EQ2.  exfalso; discriminate EQ2. 
-                   + intros A.   unfold evalSexp. intros. clear H3. clear EQ2.  hnf in H0.  rewrite EQ1 in H0.  simpl in H0. simpl  in A.  
-                     eapply  (not_zero_implies_uneq _ _  k) in H0;  eauto.   
+                   + intros.  rewrite H0 in EQ2.  exfalso; discriminate EQ2.
+                   + intros A.   unfold evalSexp. intros. clear H3. clear EQ2.  hnf in H0.  rewrite EQ1 in H0.  simpl in H0. simpl  in A.
+                     eapply  (not_zero_implies_uneq _ _  k) in H0;  eauto.
                  - split.
                    + eapply IHe1; eauto.
                    + eapply IHe2; eauto.  }
                  { rewrite H in H0; rewrite H1 in H0; simpl in H0. inversion H0. unfold binop_eval in EQ2. clear H0. unfold bvDiv in EQ2. simpl. split.
                  - case_eq(bvZero x0).
-                   + intros.  rewrite H0 in EQ2.  exfalso; discriminate EQ2. 
-                   + intros A.   unfold evalSexp. intros. clear H3. clear EQ2.  hnf in H0. rewrite EQ1 in H0.  simpl in H0. simpl  in A.  
-                     eapply ( not_zero_implies_uneq _ _ k) in H0; eauto.   
+                   + intros.  rewrite H0 in EQ2.  exfalso; discriminate EQ2.
+                   + intros A.   unfold evalSexp. intros. clear H3. clear EQ2.  hnf in H0. rewrite EQ1 in H0.  simpl in H0. simpl  in A.
+                     eapply ( not_zero_implies_uneq _ _ k) in H0; eauto.
                  -  eapply IHe1; eauto. }
                  { rewrite H in H0; rewrite H1 in H0; simpl in H0. inversion H0. unfold binop_eval in EQ2. clear H0. unfold bvDiv in EQ2. simpl. split.
                  - case_eq(bvZero x0).
-                   + intros.  rewrite H0 in EQ2.  exfalso; discriminate EQ2. 
-                   + intros A.   unfold evalSexp. intros. clear H3. clear EQ2.  hnf in H0.  rewrite EQ1 in H0.  simpl in H0. simpl  in A.  
-                     eapply  (not_zero_implies_uneq _ _ k) in H0; eauto.   
+                   + intros.  rewrite H0 in EQ2.  exfalso; discriminate EQ2.
+                   + intros A.   unfold evalSexp. intros. clear H3. clear EQ2.  hnf in H0.  rewrite EQ1 in H0.  simpl in H0. simpl  in A.
+                     eapply  (not_zero_implies_uneq _ _ k) in H0; eauto.
                  -  eapply IHe2; eauto. }
                  { rewrite H in H0; rewrite H1 in H0; simpl in H0. inversion H0. unfold binop_eval in EQ2. clear H0. unfold bvDiv in EQ2. simpl.
                    case_eq(bvZero x0).
-                   - intros.  rewrite H0 in EQ2.  exfalso; discriminate EQ2. 
-                   - intros A.   unfold evalSexp. intros. clear H3. clear EQ2.  hnf in H0. rewrite EQ1 in H0.  simpl in H0. simpl  in A.  
+                   - intros.  rewrite H0 in EQ2.  exfalso; discriminate EQ2.
+                   - intros A.   unfold evalSexp. intros. clear H3. clear EQ2.  hnf in H0. rewrite EQ1 in H0.  simpl in H0. simpl  in A.
                      eapply  (not_zero_implies_uneq _ _ k) in H0; eauto.    }
                  * case_eq (undef e1); case_eq (undef e2); intros; simpl.
                    { rewrite H in H0; rewrite H1 in H0; simpl in H0. inversion H0. simpl; split.
@@ -137,70 +121,188 @@ intros. general induction e; simpl.
       }
 Qed.
 
+Lemma ssa_eval_agree s D s' (E:onv val) (E':onv val) 
+ : ssa s D
+   -> Terminates (nil,E, s) (nil, E', s')
+   -> agree_on eq (fst (getAnn D)) E E'.
+
+Proof.
+  intros.
+  general induction H0; invt ssa; try invt F.step; simpl.
+  - reflexivity.
+  - exploit IHTerminates; [ | reflexivity | reflexivity |]; eauto.
+    rewrite H5 in X; simpl in *.
+Admitted.
+
+Lemma guardList_true_if_eval:
+forall F E el s vl,
+omap (exp_eval E) el = Some vl
+-> undefLift el = Some s
+-> models F E s.
+
+Proof.
+intros. general induction el.
+- simpl in *.  case_eq (undef a); intros.
+  + rewrite H1 in H0. simpl in H0.  case_eq (undefLift el); intros; simpl.
+    * rewrite H2 in H0. inversion H0. simpl. split.
+      { monad_inv H. eapply (guard_true_if_eval); eauto. }
+      { monad_inv H. eapply IHel; eauto. }
+    * rewrite H2 in H0. inversion H0. monad_inv H. eapply (guard_true_if_eval); eauto.
+  + rewrite H1 in H0; monad_inv H. eapply IHel; eauto.
+Qed.
+
+Lemma exp_eval_if_list_eval:
+  forall el E vl,
+    omap (exp_eval E) el = Some vl
+    -> forall e, List.In e el -> exists v, exp_eval E e = Some v.
+
+Proof.
+intros.
+general induction el. 
+- simpl in H. exists (O::nil). intros. inversion H0.
+- unfold omap in H. monad_inv H. decide (e=a).
+  + exists x. intros. rewrite e0. assumption.
+   + specialize (IHel E x0 EQ1). specialize (IHel e).  simpl in H0.  destruct H0. 
+     * exfalso. apply n. rewrite H; reflexivity. 
+     * destruct (IHel H).  exists x1.
+       rewrite H0. reflexivity.
+Qed.
+
+Lemma in_if_get:
+forall XL n  (x:exp),
+get XL n x
+-> List.In x XL.
+
+Proof. intros.
+general induction H.
+- simpl. left; eauto.
+- simpl. right. eapply IHget. reflexivity.
+Qed.
+
+Fixpoint freeVarsList el :=
+match el with
+| nil => ∅
+| e::el' => freeVars e ∪ freeVarsList el'
+end.
+
 Lemma models_if_eval :
 forall s D E s' E', 
 ssa  s D
-(*-> (forall x, x ∈ fst (getAnn D) -> E x <> None) *)
-(*-> (forall e, exists v, translateExp e = ⎣v⎦) *)
--> agree_on eq (fst (getAnn D)) E E'
+(*-> agree_on eq (fst (getAnn D)) E E' *)
 -> noFun s 
--> terminates (nil,E, s) (nil, E', s')
+-> Terminates (nil,E, s) (nil, E', s')
 ->  models (fun (f:pred) (x:vallst) => true)  E'  (translateStmt s source).
 
 Proof.
 intros.
-general induction H2; simpl.
+general induction H1; simpl.
 - assert (X: models (fun (_:pred) (_:vallst) => true) E0 (smtReturn e)).
   + simpl. econstructor.
-  + case_eq (undef e); eauto.
-    * intros. simpl; split; eauto. 
+  + case_eq (undef e); eauto; intros.
+    * simpl; split; eauto.
       eapply (guard_true_if_eval); eauto.
-- inversion H; simpl.
-  + assert (X: models (fun (_:pred) (_:vallst) => true) E' (smtAnd (constr (Var x) e) (translateStmt b source))).
-    * split; simpl.
-      {  unfold evalSexp.  
-         assert (freeVars e ⊆ fst (getAnn D)) by  (rewrite <- H7 in H0; inversion H0; simpl; assumption).  
-         assert (agree_on eq (freeVars e) E E') by (cset_tac; hnf; hnf in H1;  hnf in H9;  intros; specialize(H1 x0); specialize (H9 x0); exact (H1 (H9 H4))).
-         eapply (exp_eval_agree (E:=E) (E' := E')) in def; eauto.
-         - rewrite def. rewrite <- H7 in *. clear H7. rewrite <- H8 in *. clear H8.  simpl.
-           assert (X1:E' x = Some v).
-           + admit.
-(*           eapply (agree_on_update_dead (R:=eq) (lv:=freeVars e) (E:=E) (E':=E')(x:=x) (Some v))in H10; eauto. 
-           
-           assert ( X1: exp_eval E'  (Var x) = Some v). 
-           + eapply (exp_eval_agree (E:=E[x <-Some v]) (E':=E')).
-             * eapply agree_on_update_dead. hnf.  cset_tac. simpl in H11.  
-             * simpl. unfold update. decide (x === x).
-               { reflexivity. }
-               { exfalso; apply n; reflexivity. } *)
-           + rewrite X1.  unfold val2bool. eapply bvEq_equiv_eq. reflexivity. }
-      { rewrite <- H7 in *. inversion H0.  inversion H3. eapply IHterminates; eauto.
-        - hnf. cset_tac. admit. }
-    * case_eq (undef e); intros; eauto.
-      { simpl; split; eauto.
-        - eapply (guard_true_if_eval  (fun (_:pred) (_:vallst) => true) E' e s0 v); eauto.
-          + assert (freeVars e ⊆ fst (getAnn D)) by  (rewrite <- H7 in H0; inversion H0; simpl; assumption).  
-            assert (agree_on eq (freeVars e) E E') by (cset_tac; hnf; hnf in H1;  hnf in H10;  intros; specialize(H1 x0); specialize (H10 x0); exact (H1 (H10 H4))).
-            eapply (exp_eval_agree (E:=E) (E':=E')); eauto.
-          }
-  + assert (X: models  (fun (_:pred) (_:vallst) => true) E'( ite e (translateStmt b1 source) (translateStmt b2 source))).
-    * simpl. unfold evalSexp.   
-      assert (freeVars e ⊆ fst (getAnn D)) by  (rewrite <- H7 in H0; inversion H0; simpl; assumption).  
-      assert (agree_on eq (freeVars e) E E') by (cset_tac; hnf; hnf in H1;  hnf in H9;  intros; specialize(H1 x); specialize (H9 x); exact (H1 (H9 H4))).
+- inv H; invt ssa; invt noFun; simpl in * |- *.
+  + case_eq(undef e); intros; simpl; split; eauto.
+    * eapply (guard_true_if_eval _ E' e s v ); eauto.
+      eapply exp_eval_agree; eauto.
+      assert (A: agree_on eq (fst (getAnn (ann1 (D0, D') an))) E E').
+      { eapply (ssa_eval_agree  (stmtExp x e b) _ s'); eauto.
+        econstructor; eauto. }
+      { eapply (agree_on_incl  (bv:=Exp.freeVars e) (lv:=fst (getAnn (ann1 (D0, D') an)))); eauto. }
+    * split; eauto.
+      assert (X1: exp_eval E' (Var x) = Some v).
+      { eapply (exp_eval_agree (E:= E[x <- Some v])) ; eauto.
+        - simpl. eapply (agree_on_incl (bv:={x} ) (lv:= fst (getAnn an))).
+          + eapply (ssa_eval_agree b _ s'); eauto.
+          + rewrite H10. unfold fst. cset_tac. right; rewrite H5; reflexivity.
+        - unfold exp_eval. unfold update. decide (x===x).
+          + reflexivity.
+          + exfalso.  apply n; reflexivity. }
+      assert (X2: exp_eval E' e = Some v).
+      { eapply exp_eval_agree; eauto.
+      assert (A: agree_on eq (fst (getAnn (ann1 (D0, D') an))) E E').
+        - eapply (ssa_eval_agree  (stmtExp x e b) _ s'); eauto.
+        econstructor; eauto. 
+        - eapply (agree_on_incl  (bv:=Exp.freeVars e) (lv:=fst (getAnn (ann1 (D0, D') an)))); eauto. }
+      {  unfold evalSexp. rewrite X1; rewrite X2.
+         eapply  bvEq_equiv_eq. reflexivity.  }
+    * assert (X1: exp_eval E' (Var x) = Some v).
+      { eapply (exp_eval_agree (E:= E[x <- Some v])) ; eauto.
+        - simpl. eapply (agree_on_incl (bv:={x} ) (lv:= fst (getAnn an))).
+          + eapply (ssa_eval_agree b _ s'); eauto.
+          + rewrite H10. unfold fst. cset_tac. right; rewrite H5; reflexivity.
+        - unfold exp_eval. unfold update. decide (x===x).
+          + reflexivity.
+          + exfalso.  apply n; reflexivity. }
+      assert (X2: exp_eval E' e = Some v).
+      { eapply exp_eval_agree; eauto.
+      assert (A: agree_on eq (fst (getAnn (ann1 (D0, D') an))) E E').
+        - eapply (ssa_eval_agree  (stmtExp x e b) _ s'); eauto.
+        econstructor; eauto. 
+        - eapply (agree_on_incl  (bv:=Exp.freeVars e) (lv:=fst (getAnn (ann1 (D0, D') an)))); eauto. }
+      {  unfold evalSexp. rewrite X1; rewrite X2.
+         eapply  bvEq_equiv_eq. reflexivity.  }
+ + assert (X: models  (fun (_:pred) (_:vallst) => true) E'( ite e (translateStmt b1 source) (translateStmt b2 source))).
+    * simpl. unfold evalSexp.
+      assert (Exp.freeVars e ⊆ fst (getAnn (ann2 (D0, D') ans ant))) by (hnf; intros; hnf in H6; specialize (H6 a); exact (H6 H3)).
+      assert (agree_on eq (fst (getAnn (ann2 (D0, D') ans ant))) E E') by ( eapply (ssa_eval_agree (stmtIf e b1 b2) _ s'); eauto; econstructor; eauto). 
       erewrite (exp_eval_agree (E:=E) (E':=E')); eauto. simpl. rewrite condTrue.
       rewrite <- H7 in *.
-      inversion H0; inversion H3.
-      eapply IHterminates; eauto.
-      admit.
+      eapply IHTerminates; eauto.
+      eapply (agree_on_incl (bv:= Exp.freeVars e) (lv:= fst (getAnn (ann2 (D0, D') ans ant)))); eauto.
     * case_eq (undef e); intros; eauto.
       { simpl; split; eauto.
-        - eapply (guard_true_if_eval  (fun (_:pred) (_:vallst) => true) E' e s0 v); eauto.
-          + assert (freeVars e ⊆ fst (getAnn D)) by  (rewrite <- H7 in H0; inversion H0; simpl; assumption).  
-            assert (agree_on eq (freeVars e) E E') by (cset_tac; hnf; hnf in H1;  hnf in H10;  intros; specialize(H1 x); specialize (H10 x); exact (H1 (H10 H4))).
-            eapply (exp_eval_agree (E:=E) (E':=E')); eauto.  }
+        - eapply (guard_true_if_eval  (fun (_:pred) (_:vallst) => true) E' e _ v); eauto.
+          + assert (Exp.freeVars e ⊆ fst (getAnn (ann2 (D0, D') ans ant)))
+                   by (hnf; intros; hnf in H6; specialize (H6 a); hnf; cset_tac; simpl;  exact (H6 H4)).
+            assert (agree_on eq (fst (getAnn (ann2 (D0, D') ans ant))) E E') 
+              by ( eapply (ssa_eval_agree (stmtIf e b1 b2) _ s'); eauto; econstructor; eauto). 
+            eapply (exp_eval_agree (E:=E) (E':=E')); eauto.
+            eapply (agree_on_incl (bv:= Exp.freeVars e) (lv:= fst (getAnn (ann2 (D0, D') ans ant)))); eauto.
+      }
+ + assert (X: models  (fun (_:pred) (_:vallst) => true) E'( ite e (translateStmt b1 source) (translateStmt b2 source))).
+    * simpl. unfold evalSexp.
+      assert (Exp.freeVars e ⊆ fst (getAnn (ann2 (D0, D') ans ant))) by (hnf; intros; hnf in H6; specialize (H6 a); exact (H6 H3)).
+      assert (agree_on eq (fst (getAnn (ann2 (D0, D') ans ant))) E E') by ( eapply (ssa_eval_agree (stmtIf e b1 b2) _ s'); eauto; econstructor; eauto). 
+      erewrite (exp_eval_agree (E:=E) (E':=E')); eauto. simpl. rewrite condFalse.
+      rewrite <- H7 in *.
+      eapply IHTerminates; eauto.
+      eapply (agree_on_incl (bv:= Exp.freeVars e) (lv:= fst (getAnn (ann2 (D0, D') ans ant)))); eauto.
+    * case_eq (undef e); intros; eauto.
+      { simpl; split; eauto.
+        - eapply (guard_true_if_eval  (fun (_:pred) (_:vallst) => true) E' e _ v); eauto.
+          + assert (Exp.freeVars e ⊆ fst (getAnn (ann2 (D0, D') ans ant)))
+                   by (hnf; intros; hnf in H6; specialize (H6 a); hnf; cset_tac; simpl;  exact (H6 H4)).
+            assert (agree_on eq (fst (getAnn (ann2 (D0, D') ans ant))) E E') 
+              by ( eapply (ssa_eval_agree (stmtIf e b1 b2) _ s'); eauto; econstructor; eauto). 
+            eapply (exp_eval_agree (E:=E) (E':=E')); eauto.
+            eapply (agree_on_incl (bv:= Exp.freeVars e) (lv:= fst (getAnn (ann2 (D0, D') ans ant)))); eauto.
+      }
+ + admit.
+(*
++ case_eq (undefLift Y); intros; simpl; eauto.
+    *  split; eauto.  eapply (guardList_true_if_eval); eauto.
+       assert ( list_union (List.map freeVars  Y)  ⊆ fst (getAnn D)) by ( rewrite <- H7 in H0; inversion H0; simpl; assumption).
+       assert (agree_on eq (list_union (List.map freeVars Y)) E E') by (cset_tac; hnf; hnf in H1;  hnf in H10;  intros; specialize(H1 x); specialize (H10 x); exact (H1 (H10 H4))).
+       erewrite omap_agree; eauto.
+       intros. 
+       destruct Y. 
+       { inversion H12. }
+       { assert (X: exists v, (exp_eval E x) = Some v).
+         - eapply exp_eval_if_list_eval; eauto. eapply in_if_get; eauto. 
+         - destruct X.  rewrite H13.
+         assert (freeVars x ⊆ fst (getAnn D)).
+           +  cset_tac. hnf in H10. specialize (H10 a). eapply H10.  unfold list_union.  simpl.  eapply list_union_start_swap.  cset_tac. left; right; assumption. 
+         - assert (agree_on eq (freeVars x) E E'). 
+           + cset_tac. hnf.  hnf in H11.  intros. eapply (H11 x2). unfold list_union. simpl. eapply list_union_start_swap. cset_tac.  left;right; assumption.
+           + eapply exp_eval_agree; eauto. }
+*)
+Qed.
+
+(*
   +  assert (X: models  (fun (_:pred) (_:vallst) => true) E'( ite e (translateStmt b1 source) (translateStmt b2 source))).
-    * simpl. unfold evalSexp.   
-      assert (freeVars e ⊆ fst (getAnn D)) by  (rewrite <- H7 in H0; inversion H0; simpl; assumption).  
+    * simpl. unfold evalSexp.
+      assert (freeVars e ⊆ fst (getAnn D)) by  (rewrite <- H7 in H0; inversion H0; simpl; assumption).
       assert (agree_on eq (freeVars e) E E') by (cset_tac; hnf; hnf in H1;  hnf in H9;  intros; specialize(H1 x); specialize (H9 x); exact (H1 (H9 H4))).
       erewrite (exp_eval_agree (E:=E) (E':=E')); eauto. simpl. rewrite condFalse.
       rewrite <- H7 in *.
@@ -210,15 +312,147 @@ general induction H2; simpl.
     * case_eq (undef e); intros; eauto.
       { simpl; split; eauto.
         - eapply (guard_true_if_eval  (fun (_:pred) (_:vallst) => true) E' e s0 v); eauto.
-          + assert (freeVars e ⊆ fst (getAnn D)) by  (rewrite <- H7 in H0; inversion H0; simpl; assumption).  
+          + assert (freeVars e ⊆ fst (getAnn D)) by  (rewrite <- H7 in H0; inversion H0; simpl; assumption).
             assert (agree_on eq (freeVars e) E E') by (cset_tac; hnf; hnf in H1;  hnf in H10;  intros; specialize(H1 x); specialize (H10 x); exact (H1 (H10 H4))).
             eapply (exp_eval_agree (E:=E) (E':=E')); eauto.  }
-  + general induction Y; intros.
+(* exploit IHTerminates; [ | |reflexivity | reflexivity |   ]; eauto.
+    exploit ssa_eval_agree; try eapply H1; eauto.
+    case_eq (undef e); intros; simpl; split; eauto.
+    * eapply guard_true_if_eval; eauto.
+      eapply (exp_eval_agree (E:=E) (E':=E') _ (v:=Some v) ).
+      { eapply (agree_on_incl (lv:= fst(getAnn an)) ); eauto. 
+        eapply ssa_eval_agree; eauto.
+        - eapply agree_on_incl; eauto.
+      rewrite H10. simpl. rewrite H7. cset_tac; intuition.
+      (* E [x <- Some v] and E agree on freeVars e *) exfalso; admit.
+    * split.
+      unfold evalSexp.
+      erewrite exp_eval_agree; eauto.
+      instantiate (1:=E[x <- Some v]).
+      setoid_rewrite exp_eval_agree at 2.
+      Focus 2. instantiate (1:=E[x <- Some v]). admit.
+      Focus 2. instantiate (1:=exp_eval E e). admit.
+      simpl. lud. rewrite def. eapply bvEq_equiv_eq; reflexivity.
+      isabsurd. admit.
+      eauto.
+   * admit. *)
+(*  + assert (X: models (fun (_:pred) (_:vallst) => true) E' (smtAnd (constr (Var x) e) (translateStmt b source))).
+    * split; simpl.
+      {  unfold evalSexp.
+         assert (freeVars e ⊆ fst (getAnn D)) by  (rewrite <- H7 in H0; inversion H0; simpl; assumption).
+         assert (agree_on eq (freeVars e) E E') by (cset_tac; hnf; hnf in H1;  hnf in H9;  intros; specialize(H1 x0); specialize (H9 x0); exact (H1 (H9 H4))).
+         eapply (exp_eval_agree (E:=E) (E' := E')) in def; eauto.
+         - rewrite def. rewrite <- H7 in *. clear H7. rewrite <- H8 in *. clear H8.  simpl.
+           assert (X1:E' x = Some v).
+           + admit.
+(*           eapply (agree_on_update_dead (R:=eq) (lv:=freeVars e) (E:=E) (E':=E')(x:=x) (Some v))in H10; eauto.
+
+           assert ( X1: exp_eval E'  (Var x) = Some v).
+           + eapply (exp_eval_agree (E:=E[x <-Some v]) (E':=E')).
+             * eapply agree_on_update_dead. hnf.  cset_tac. simpl in H11.
+             * simpl. unfold update. decide (x === x).
+               { reflexivity. }
+               { exfalso; apply n; reflexivity. } *)
+           + rewrite X1.  unfold val2bool. eapply bvEq_equiv_eq. reflexivity. }
+      { rewrite <- H7 in *. inversion H0.  inversion H3. eapply IHterminates; eauto.
+        - hnf. cset_tac. admit. }
+    * case_eq (undef e); intros; eauto.
+      { simpl; split; eauto.
+        - eapply (guard_true_if_eval  (fun (_:pred) (_:vallst) => true) E' e s0 v); eauto.
+          + assert (freeVars e ⊆ fst (getAnn D)) by  (rewrite <- H7 in H0; inversion H0; simpl; assumption).
+            assert (agree_on eq (freeVars e) E E') by (cset_tac; hnf; hnf in H1;  hnf in H10;  intros; specialize(H1 x0); specialize (H10 x0); exact (H1 (H10 H4))).
+            eapply (exp_eval_agree (E:=E) (E':=E')); eauto.
+          } *)
+  + assert (X: models  (fun (_:pred) (_:vallst) => true) E'( ite e (translateStmt b1 source) (translateStmt b2 source))).
+    * simpl. unfold evalSexp.
+      assert (Exp.freeVars e ⊆ fst (getAnn (ann2 (D0, D') ans ant))) by  (rewrite <- H7 in H0; inversion H0; simpl; assumption). 
+      assert (agree_on eq (freeVars e) E E') by (cset_tac; hnf; hnf in H1;  hnf in H9;  intros; specialize(H1 x); specialize (H9 x); exact (H1 (H9 H4))).
+      erewrite (exp_eval_agree (E:=E) (E':=E')); eauto. simpl. rewrite condTrue.
+      rewrite <- H7 in *.
+      inversion H0; inversion H3.
+      eapply IHterminates; eauto.
+      admit.
+    * case_eq (undef e); intros; eauto.
+      { simpl; split; eauto.
+        - eapply (guard_true_if_eval  (fun (_:pred) (_:vallst) => true) E' e s0 v); eauto.
+          + assert (freeVars e ⊆ fst (getAnn D)) by  (rewrite <- H7 in H0; inversion H0; simpl; assumption).
+            assert (agree_on eq (freeVars e) E E') by (cset_tac; hnf; hnf in H1;  hnf in H10;  intros; specialize(H1 x); specialize (H10 x); exact (H1 (H10 H4))).
+            eapply (exp_eval_agree (E:=E) (E':=E')); eauto.  }
+  +  assert (X: models  (fun (_:pred) (_:vallst) => true) E'( ite e (translateStmt b1 source) (translateStmt b2 source))).
+    * simpl. unfold evalSexp.
+      assert (freeVars e ⊆ fst (getAnn D)) by  (rewrite <- H7 in H0; inversion H0; simpl; assumption).
+      assert (agree_on eq (freeVars e) E E') by (cset_tac; hnf; hnf in H1;  hnf in H9;  intros; specialize(H1 x); specialize (H9 x); exact (H1 (H9 H4))).
+      erewrite (exp_eval_agree (E:=E) (E':=E')); eauto. simpl. rewrite condFalse.
+      rewrite <- H7 in *.
+      inversion H0; inversion H3.
+      eapply IHterminates; eauto.
+      admit.
+    * case_eq (undef e); intros; eauto.
+      { simpl; split; eauto.
+        - eapply (guard_true_if_eval  (fun (_:pred) (_:vallst) => true) E' e s0 v); eauto.
+          + assert (freeVars e ⊆ fst (getAnn D)) by  (rewrite <- H7 in H0; inversion H0; simpl; assumption).
+            assert (agree_on eq (freeVars e) E E') by (cset_tac; hnf; hnf in H1;  hnf in H10;  intros; specialize(H1 x); specialize (H10 x); exact (H1 (H10 H4))).
+            eapply (exp_eval_agree (E:=E) (E':=E')); eauto.  }
++ case_eq (undefLift Y); intros; simpl; eauto.
+    *  split; eauto.  eapply (guardList_true_if_eval); eauto.
+       assert ( list_union (List.map freeVars  Y)  ⊆ fst (getAnn D)) by ( rewrite <- H7 in H0; inversion H0; simpl; assumption).
+       assert (agree_on eq (list_union (List.map freeVars Y)) E E') by (cset_tac; hnf; hnf in H1;  hnf in H10;  intros; specialize(H1 x); specialize (H10 x); exact (H1 (H10 H4))).
+       erewrite omap_agree; eauto.
+       intros. 
+       destruct Y. 
+       { inversion H12. }
+       { assert (X: exists v, (exp_eval E x) = Some v).
+         - eapply exp_eval_if_list_eval; eauto. eapply in_if_get; eauto. 
+         - destruct X.  rewrite H13.
+         assert (freeVars x ⊆ fst (getAnn D)).
+           +  cset_tac. hnf in H10. specialize (H10 a). eapply H10.  unfold list_union.  simpl.  eapply list_union_start_swap.  cset_tac. left; right; assumption. 
+         - assert (agree_on eq (freeVars x) E E'). 
+           + cset_tac. hnf.  hnf in H11.  intros. eapply (H11 x2). unfold list_union. simpl. eapply list_union_start_swap. cset_tac.  left;right; assumption.
+           + eapply exp_eval_agree; eauto. }
+
+ destruct H12.
+       { unfold omap in def. monad_inv def. rewrite EQ.
+         assert (freeVars x ⊆ fst (getAnn D)).
+         -  cset_tac. hnf in H10. specialize (H10 a). eapply H10.  unfold list_union.  simpl.  eapply list_union_start_swap.  cset_tac. left; right; assumption. 
+         - assert (agree_on eq (freeVars x) E E'). 
+           + cset_tac. hnf.  hnf in H11.  intros. eapply (H11 x2). unfold list_union. simpl. eapply list_union_start_swap. cset_tac.  left;right; assumption.
+           + eapply exp_eval_agree; eauto. }
+       { assert (X: exists v, (exp_eval E x) = Some v).
+         - eapply  exp_eval_if_list_eval; eauto. 
+           + cset_tac. hnf. right. hnf. left; reflexivity.
+           + decide (x = x'0).
+             * hnf. left; eauto.
+             * hnf. right. eapply IHget; eauto.
+           
+         - eapply exp_eval_if_list_eval.   }
+(*intros. 
+       unfold omap in def. eapply (omap_inversion _ _ (exp_eval E) Y) . assumption.
+        { inversion H12.  }
+        { inversion H12.  rewrite <- H16.  monad_inv def.  rewrite EQ. 
+         assert (freeVars x ⊆ fst (getAnn D)).
+         -  cset_tac. hnf in H10. specialize (H10 a). eapply H10.  unfold list_union.  simpl.  eapply list_union_start_swap.  cset_tac. left; right; assumption. 
+         - assert (agree_on eq (freeVars x) E E'). 
+           + cset_tac. hnf.  hnf in H11.  intros. eapply (H11 x0). unfold list_union. simpl. eapply list_union_start_swap. cset_tac.  left;right; assumption.
+           + eapply exp_eval_agree; eauto. 
+         - eapply exp_eval_if_list_eval.   }
+             
+           cset_tac; hnf; hnf in H1;  hnf in H10;  intros; specialize(H1 x); specialize (H10 x); exact (H1 (H10 H4)).
+         eapply (exp_eval_agree (E:=E) (E':=E')); eauto.
+eapply exp_eval_agree.
+         
+       { simpl in def. monad_inv def.  
+}
+       { simpl in H9.  case_eq (undef a); intros; simpl.
+         - eapply IHY; eauto.
+       { simpl  in H9. unfold omap in def. monad_inv def.  case_eq (undef a0); intros.
+         - 
     * simpl. econstructor.
-    * admit. (* TODO: Build List Lemma from guard_true_if_eval *)
+    * simpl. case_eq (undefLift (a
+      { simpl. split; eapply IHY;  admit. (* TODO: Build List Lemma from guard_true_if_eval *) *) admit.
   + rewrite <-  H7 in H3. exfalso. inversion H3.
   + rewrite <- H7 in H3. exfalso. inversion H3.
 Qed.
+*)
 
 Definition smtCheck (s:stmt) (t:stmt) :=
 smtAnd (translateStmt s source) (translateStmt t target).
@@ -245,18 +479,32 @@ forall s t F E XL YL,
 ~ (models F E (smtCheck s t))
 -> noFun s
 -> noFun t
--> OutVars XL s
--> OutVars YL t
-->List.length XL = List.length YL
 -> (forall F V,  models F V (translateStmt s source) -> models F V (translateStmt t source))
--> agreeOnList E (List.length XL) XL YL.
+-> sim s t
 
 Proof.
-intros. general induction s.
+admit.
+(*intros. general induction s.
 - general induction t.
-  + 
+  +  *)
 Qed.
 
+(** Checks wether two lists agree on their values. But the environment needs to be defined on every
+variable. Otherwise the result is false **)
+Fixpoint agreeOnList' (k:nat)E1 E2 XL YL:=
+match k with
+| 0 => True
+| S k' =>  match XL, YL with
+             |nil , nil => True
+             | nil, _ => False
+             | _, nil => False
+             | a::XL', b::YL' => match (exp_eval E1 a), (exp_eval E2 b) with
+                                   | Some v1, Some v2 => v1 = v2 /\ (agreeOnList' k'  E1 E2 XL' YL')
+                                   | None, None =>  False
+                                   | _,_ => False
+                                 end
+           end
+end.
 Lemma unsat_is_semeq :
 forall s t s' t' E E1 E2 XL YL,
 terminates (nil, E , s) (nil, E1, s')
@@ -265,10 +513,11 @@ terminates (nil, E , s) (nil, E1, s')
 -> OutVars YL t
 -> noFun s
 -> noFun t
--> agreeOnList E (List.length XL) XL YL.
+-> (forall F E, ~ models F E (smtCheck s t))
+-> agreeOnList'  (List.length XL) E1 E2 XL YL.
 
 Proof.
-admit.
+intros. unfold smtCheck in H5. simpl in H5.  admit.
 Qed.
 
 (*
